Fixes regarding indexing of Stable Checkpoints.
* SequenceID data type starts form 0, but we start committing from 1.
  This way we start with LastStableCkeckpoint at 0 and commit beyond it.
* Fix for CheckpointsQuorum's valid predicate to take in consideration
  that for Sequence ID 0 we don't need agreement quorum of Checkpoint messages.
* Added checked predicate for ViewChangeMsg and NewViewMsg which does all necessary
  checks including the signature checking, which is achieved on the call site by
  passing all the messages the network has stored. The call sites in replica.i.dfy
  have been revised.
* Fix to set the lastStableCheckpoint == 0 in replica.i.dfy's Init predicate.
* proof.dfy has been revised to take in consideration the above changes + hints
  on the lemmas that need to be completed.

docs/sbft-formal-model/messages.dfy
@@ -11,13 +11,15 @@
 
 include "network.s.dfy"
 include "library/Library.dfy"
+include "cluster_config.s.dfy"
 
 module Messages {
   import Library
   import opened HostIdentifiers
   import Network
+  import ClusterConfig
 
-  type SequenceID = k:nat | 0 < k witness 1
+  type SequenceID = nat
   type ViewNum = nat
 
   datatype ClientOperation = ClientOperation(sender:HostId, timestamp:nat)
@@ -72,12 +74,14 @@ module Messages {
       prot.payload
     }
     predicate valid(lastStableCheckpoint:SequenceID, quorumSize:nat) {
-      && |msgs| > 0
-      && UniqueSenders(msgs)
-      && (forall m | m in msgs :: && m.payload.CheckpointMsg?
-                                  && m.payload == prototype()
-                                  && m.payload.seqIDReached == lastStableCheckpoint)
-      && |msgs| >= quorumSize
+      || (&& lastStableCheckpoint == 0
+          && |msgs| == 0)
+      || (&& |msgs| > 0
+          && UniqueSenders(msgs)
+          && (forall m | m in msgs :: && m.payload.CheckpointMsg?
+                                      && m.payload == prototype()
+                                      && m.payload.seqIDReached == lastStableCheckpoint)
+          && |msgs| >= quorumSize)
     }
   }
 
@@ -105,6 +109,12 @@ module Messages {
                          && (ViewChangeMsg? ==> validViewChangeMsg(quorumSize))
                          && (NewViewMsg? ==> validNewViewMsg(quorumSize))
                        }
+                       predicate checked(clusterConfig:ClusterConfig.Constants, sigChecks:set<Network.Message<Message>>)
+                         requires clusterConfig.WF()
+                       {
+                         && (ViewChangeMsg? ==> checkedViewChangeMsg(clusterConfig, sigChecks))
+                         && (NewViewMsg? ==> checkedNewViewMsg(clusterConfig, sigChecks))
+                       }
                        predicate validViewChangeMsg(quorumSize:nat) 
                          requires ViewChangeMsg?
                        {
@@ -114,6 +124,28 @@ module Messages {
                          requires NewViewMsg?
                        {
                          vcMsgs.valid(newView, quorumSize)
+                       }
+                       predicate checkedViewChangeMsg(clusterConfig:ClusterConfig.Constants, sigChecks:set<Network.Message<Message>>)
+                         requires ViewChangeMsg?
+                         requires clusterConfig.WF()
+                       {
+                          && valid(clusterConfig.AgreementQuorum())
+                          // Check Checkpoint msg-s signatures:
+                          && proofForLastStable.msgs <= sigChecks
+                          && (forall seqID | seqID in certificates
+                                  :: && certificates[seqID].votes <= sigChecks
+                                     && (forall replica | replica in sendersOf(certificates[seqID].votes)
+                                                      :: clusterConfig.IsReplica(replica))
+                                     && certificates[seqID].valid(clusterConfig.AgreementQuorum(), seqID))
+                       }
+                       predicate checkedNewViewMsg(clusterConfig:ClusterConfig.Constants, sigChecks:set<Network.Message<Message>>)
+                         requires NewViewMsg?
+                         requires clusterConfig.WF()
+                       {
+                          && valid(clusterConfig.AgreementQuorum())
+                          && (forall replica | replica in sendersOf(vcMsgs.msgs)
+                                               :: clusterConfig.IsReplica(replica))
+                          && vcMsgs.msgs <= sigChecks
                        }
                        predicate IsIntraViewMsg() {
                           || PrePrepare?
